providers/evercrypt/fst/EverCrypt.Hash.fst
@@ -175,7 +175,6 @@ let update_multi #a s blocks len =
 
 // Re-using the higher-order stateful combinator to get an instance of
 // update_last that is capable of calling Vale under the hood
-val update_last_256: Hacl.Hash.Definitions.update_last_st SHA2_256
 let update_last_256 s prev_len input input_len =
   Hacl.Hash.MD.mk_update_last SHA2_256 update_multi_256 Hacl.Hash.SHA2.pad_256 s prev_len input input_len
 
